Phi_System/IDE_CP_Applications1.thy
@@ -805,7 +805,7 @@ structure PhiDef_SS = Simpset (
 )\<close>
 
 \<phi>reasoner_ML Unfold_\<phi>Defs 1000 (\<open>Unfold_\<phi>Defs ?X' ?X\<close>)
-  = \<open>Phi_Reasoners.wrap (PLPR_Simplifier.simplifier_by_ss' PhiDef_SS.get')\<close>
+  = \<open>Phi_Reasoners.wrap (PLPR_Simplifier.simplifier_by_ss' (K Seq.empty) PhiDef_SS.get')\<close>
 
 declare prod.case[\<phi>defs]
 
